wrote a complete spec for is_elem and proved it is correct

examples/heapster/linked_list_proofs.v
@@ -16,10 +16,10 @@ Import SAWCorePrelude.
 
 Lemma no_errors_is_elem : refinesFun is_elem (fun _ _ => noErrorsSpec).
 Proof.
-  prove_refinesFun.
+  prove_refinement.
 Qed.
 
-Lemma no_errors_is_elem_manual : refinesFun is_elem (fun _ _ => noErrorsSpec).a
+Lemma no_errors_is_elem_manual : refinesFun is_elem (fun _ _ => noErrorsSpec).
 Proof.
   unfold noErrorsSpec.
   apply refinesFun_multiFixM_fst. intros x l.
@@ -33,4 +33,40 @@ Proof.
       apply refinesM_existsM_l; intros. rewrite returnM_bindM.
       apply refinesM_sigT_rect_l; intros.
       eapply refinesM_existsM_r. reflexivity.
+Qed.
+
+
+Fixpoint is_elem_spec (x:bitvector 64) (l:W64List) : CompM {_:bitvector 64 & unit} :=
+  match l with
+  | W64Nil => returnM (existT _ (bvNat 64 0) tt)
+  | W64Cons y l' =>
+    if bvEq 64 x y then returnM (existT _ (bvNat 64 1) tt) else
+      is_elem_spec x l'
+  end.
+
+(* Arguments is_elem_spec /. *)
+
+Lemma bvEq_sym n x y : bvEq n x y = bvEq n y x.
+  admit.
+Admitted.
+
+From Coq Require Import Nat.
+
+Lemma bvEq_eqb n x y : bvEq n (bvNat n x) (bvNat n y) = eqb x y.
+  admit.
+Admitted.
+
+Lemma is_elem_correct : refinesFun is_elem is_elem_spec.
+Proof.
+  prove_refinesFun.
+  induction a0; unfold is_elem_spec; simpl; prove_refinement.
+  - rewrite bvEq_sym in H. rewrite H in * |- *.
+    rewrite bvEq_eqb in H0. discriminate H0.
+  - rewrite bvEq_sym in H. rewrite H in * |- *.
+    rewrite bvEq_eqb in H0. discriminate H0.
+  - transitivity (is_elem_spec a a0 >>= returnM);
+      [ | rewrite bindM_returnM; reflexivity ].
+    apply Proper_refinesM_bindM; [ reflexivity | ].
+    intros sig1 sig2 esig; rewrite esig.
+    destruct sig2; simpl. destruct u. reflexivity.
 Qed.
